proof/invariant-abstract/Schedule_AI.thy
@@ -164,6 +164,401 @@ lemma invs_upd_cur_valid:
   by (fastforce simp: valid_def invs_def valid_state_def cur_tcb_def valid_machine_state_def)
 
 
+(* RT: sc_and_timer invs *)
+
+lemma set_refills_valid_objs:
+  "\<lbrace>valid_objs and K (length refills \<ge> 1)\<rbrace>
+    set_refills sc_ptr refills \<lbrace>\<lambda>rv. valid_objs\<rbrace>"
+  apply (wpsimp simp: set_refills_def valid_objs_def valid_obj_def
+                 wp: get_sched_context_wp)
+  apply (drule_tac x=sc_ptr in bspec)
+  apply (fastforce simp: obj_at_def)
+  by (auto simp: obj_at_def valid_sched_context_def)
+
+crunches commit_domain_time,set_next_interrupt,set_refills,refill_split_check
+  for consumed_time[wp]: "\<lambda>s. P (consumed_time s)"
+  and reprogram_timer[wp]: "\<lambda>s. P (reprogram_timer s)"
+  and cur_sc[wp]: "\<lambda>s. P (cur_sc s)"
+  and cur_time[wp]: "\<lambda>s. P (cur_time s)"
+  and cur_thread[wp]: "\<lambda>s. P (cur_thread s)"
+  and cur_sc_cur_thread[wp]: "\<lambda>s. P (cur_sc s) (cur_thread s)"
+  (wp: crunch_wps simp: Let_def)
+
+crunch reprogram_timer[wp]: commit_time "\<lambda>s. P (reprogram_timer s)"
+  (wp: crunch_wps hoare_vcg_if_lift2 ignore: commit_domain_time)
+
+lemma refill_unblock_check_reprogram_timer[wp]:
+  "\<lbrace>\<lambda>s. \<forall>b. P b\<rbrace> refill_unblock_check param_a \<lbrace>\<lambda>_ s. P (reprogram_timer s)\<rbrace>"
+  by (wpsimp simp: refill_unblock_check_def wp: crunch_wps hoare_vcg_if_lift2)
+
+crunches refill_unblock_check
+  for consumed_time[wp]: "\<lambda>s. P (consumed_time s)"
+  and cur_sc[wp]: "\<lambda>s. P (cur_sc s)"
+  and cur_time[wp]: "\<lambda>s. P (cur_time s)"
+  and cur_sc_cur_thread[wp]: "\<lambda>s. P (cur_sc s) (cur_thread s)"
+  (wp: crunch_wps hoare_vcg_if_lift2)
+
+lemma rollback_time_consumed_time[wp]:
+  "\<lbrace>\<lambda>s. \<forall>b. P b\<rbrace> rollback_time \<lbrace>\<lambda>_ s. P (consumed_time s)\<rbrace>"
+  by (wpsimp simp: rollback_time_def)
+
+lemma cur_time_consumed_time[wp]:
+  "\<lbrace>\<lambda>s. \<forall>b. P b\<rbrace> rollback_time \<lbrace>\<lambda>_ s. P (cur_time s)\<rbrace>"
+  by (wpsimp simp: rollback_time_def)
+
+lemma rollback_time_cur_time[wp]:
+  "\<lbrace>\<lambda>s. \<forall>a b. P a b\<rbrace> rollback_time \<lbrace>\<lambda>_ s. P (cur_time s) (consumed_time s)\<rbrace>"
+  by (wpsimp simp: rollback_time_def wp: hoare_drop_imp)
+
+lemma commit_time_consumed_time[wp]:
+  "\<lbrace>\<lambda>s. \<forall>b. P b\<rbrace> commit_time \<lbrace>\<lambda>_ s. P (consumed_time s)\<rbrace>"
+  by (wpsimp simp: commit_time_def)
+
+crunches sc_and_timer
+  for consumed_time[wp]: "\<lambda>s. P (consumed_time s)"
+  and reprogram_timer[wp]: "\<lambda>s. P (reprogram_timer s)"
+  (wp: crunch_wps hoare_vcg_if_lift2 ignore: set_next_interrupt)
+
+lemma valid_sc_valid_refills:
+   "\<lbrakk>valid_objs s; kheap s sc_ptr = Some (SchedContext sc n) \<rbrakk>
+         \<Longrightarrow> length (sc_refills sc) \<ge> 1"
+  by (fastforce simp: valid_objs_def valid_obj_def valid_sched_context_def)
+
+lemma round_robin_inv[wp]: "\<lbrace>\<lambda>s. P s\<rbrace> is_round_robin x \<lbrace> \<lambda>_ s. P s\<rbrace>"
+  by (wpsimp simp: is_round_robin_def)
+
+lemma get_sched_context_sp:
+  "\<lbrace>P\<rbrace> get_sched_context sc_ptr
+   \<lbrace> \<lambda>r s. P s \<and> (\<exists>n. ko_at (SchedContext r n) sc_ptr s)\<rbrace>"
+  apply (simp add: get_sched_context_def)
+  apply (rule hoare_seq_ext[rotated])
+   apply (rule get_object_sp)
+  apply (wpsimp, fastforce)
+  done
+
+lemma get_refills_sp:
+  "\<lbrace>P\<rbrace> get_refills sc_ptr
+  \<lbrace> \<lambda>r s. P s \<and> (\<exists>sc n. ko_at (SchedContext sc n) sc_ptr s \<and> r = sc_refills sc)\<rbrace>"
+  apply (simp add: get_refills_def)
+  apply (rule hoare_seq_ext[rotated])
+   apply (rule get_sched_context_sp)
+  apply (wp hoare_return_sp)
+  apply clarsimp
+  apply (rule_tac x=sc in exI, auto)
+  done
+
+lemma get_refills_wp:
+  "\<lbrace>\<lambda>s. \<forall>r sc n. (ko_at (SchedContext sc n) sc_ptr s \<and> r = sc_refills sc) \<longrightarrow> P r s\<rbrace>
+     get_refills sc_ptr
+  \<lbrace> \<lambda>r s. P r s\<rbrace>"
+  by (wpsimp simp: get_sched_context_def get_refills_def wp: get_object_wp) fastforce
+
+lemma refills_merge_valid:
+  "length ls \<ge> 1 \<Longrightarrow> 1 \<le> length (refills_merge_prefix ls)"
+  apply (induct ls rule: refills_merge_prefix.induct)
+  by (fastforce simp add: valid_sched_context_def)+
+
+lemma refill_unblock_check_valid_objs[wp]:
+  "\<lbrace>valid_objs and sc_at sc_ptr\<rbrace> refill_unblock_check sc_ptr \<lbrace>\<lambda>rv. valid_objs\<rbrace>"
+  apply (rule hoare_assume_pre)
+  apply (clarsimp simp: pred_def obj_at_def is_sc_obj_def)
+  apply (case_tac ko; clarsimp simp:)
+  apply (rename_tac sc n)
+  apply (frule (1) valid_sc_valid_refills[rotated])
+  apply (wpsimp wp: get_sched_context_wp get_refills_wp set_refills_valid_objs
+      hoare_vcg_conj_lift hoare_drop_imp hoare_vcg_if_lift2
+      simp: pred_conj_def refill_unblock_check_def obj_at_def is_sc_obj_def
+      split: kernel_object.splits)
+  apply (frule_tac sc=sca in valid_sc_valid_refills[rotated], simp)
+  apply (case_tac "sc_refills sca", simp)
+  apply simp
+  apply (auto simp: refills_merge_valid[simplified])
+  done
+
+lemma refill_split_check_valid_objs[wp]:
+  "\<lbrace>valid_objs and sc_at sc_ptr\<rbrace> refill_split_check sc_ptr usage \<lbrace>\<lambda>rv. valid_objs\<rbrace>"
+  apply (rule hoare_assume_pre)
+  apply (clarsimp simp: pred_def obj_at_def is_sc_obj_def)
+  apply (case_tac ko; clarsimp simp:)
+  apply (rename_tac sc n)
+  apply (frule (1) valid_sc_valid_refills[rotated])
+  apply (wpsimp wp: get_sched_context_wp get_refills_sp set_refills_valid_objs
+      hoare_vcg_conj_lift hoare_drop_imp hoare_vcg_if_lift2
+      simp: pred_conj_def refill_split_check_def obj_at_def is_sc_obj_def Let_def
+      split: kernel_object.splits split_del: if_splits)
+  apply (frule_tac sc=sca in valid_sc_valid_refills[rotated], simp)
+  apply (case_tac "sc_refills sca", simp)
+  apply (auto simp: refills_merge_valid[simplified])
+  done
+
+(* move to KHeap_AI *)
+crunch valid_irq_states[wp]: update_sched_context "valid_irq_states"
+  (wp: crunch_wps simp: crunch_simps)
+
+(* move to Invariants_AI *)
+lemma valid_irq_states_consumed_time_update[iff]:
+  "valid_irq_states (consumed_time_update f s) = valid_irq_states s"
+  by (simp add: valid_irq_states_def)
+lemma vms_consumed_time_update[iff]:
+  "valid_machine_state (consumed_time_update f s) = valid_machine_state s"
+  by (simp add: valid_machine_state_def)
+
+(* move to Invariants_AI *)
+lemma valid_irq_states_cur_time_update[iff]:
+  "valid_irq_states (cur_time_update f s) = valid_irq_states s"
+  by (simp add: valid_irq_states_def)
+lemma vms_cur_time_update[iff]:
+  "valid_machine_state (cur_time_update f s) = valid_machine_state s"
+  by (simp add: valid_machine_state_def)
+
+(* move to Invariants_AI *)
+lemma valid_irq_states_reprogram_timer_update[iff]:
+  "valid_irq_states (reprogram_timer_update f s) = valid_irq_states s"
+  by (simp add: valid_irq_states_def)
+lemma vms_reprogram_timer_update[iff]:
+  "valid_machine_state (reprogram_timer_update f s) = valid_machine_state s"
+  by (simp add: valid_machine_state_def)
+
+(* move to Invariants_AI *)
+lemma valid_irq_states_cur_sc_update[iff]:
+  "valid_irq_states (cur_sc_update f s) = valid_irq_states s"
+  by (simp add: valid_irq_states_def)
+lemma vms_cur_c_update[iff]:
+  "valid_machine_state (cur_sc_update f s) = valid_machine_state s"
+  by (simp add: valid_machine_state_def)
+
+(* move to ArchAcc_AI? *)
+lemma cur_tcb_consumed_time_update[iff]:
+  "cur_tcb (consumed_time_update f s) = cur_tcb s"
+  by (simp add: cur_tcb_def)
+
+(* move to ArchAcc_AI? *)
+lemma cur_tcb_cur_time_update[iff]:
+  "cur_tcb (cur_time_update f s) = cur_tcb s"
+  by (simp add: cur_tcb_def)
+
+(* move to ArchAcc_AI? *)
+lemma cur_tcb_cur_sc_update[iff]:
+  "cur_tcb (cur_sc_update f s) = cur_tcb s"
+  by (simp add: cur_tcb_def)
+
+(* move to ArchAcc_AI? *)
+lemma cur_tcb_reprogram_timer_update[iff]:
+  "cur_tcb (reprogram_timer_update f s) = cur_tcb s"
+  by (simp add: cur_tcb_def)
+
+lemma refs_of_sc_consumed_update[iff]:
+  "refs_of_sc (sc_consumed_update f sc) = refs_of_sc sc"
+  by simp
+
+lemma refs_of_sc_refills_update[iff]:
+  "refs_of_sc (sc_refills_update f sc) = refs_of_sc sc"
+  by simp
+
+lemma refs_of_sched_context_sc_consumed_update[iff]:
+  "refs_of (SchedContext (sc_consumed_update f sc) n) = refs_of (SchedContext sc n)"
+  by simp
+
+lemma refs_of_sched_context_sc_refills_update[iff]:
+  "refs_of (SchedContext (sc_refills_update f sc) n) = refs_of (SchedContext sc n)"
+  by simp
+
+lemma sc_consumed_update_iflive [wp]:
+  "\<lbrace>\<lambda>s. if_live_then_nonz_cap s \<and> (live_sc sc \<longrightarrow> ex_nonz_cap_to ptr s)\<rbrace>
+     update_sched_context ptr (sc_consumed_update f sc) \<lbrace>\<lambda>rv. if_live_then_nonz_cap\<rbrace>"
+  by (wpsimp simp: live_sc_def)
+
+lemma sc_refills_update_iflive [wp]:
+  "\<lbrace>\<lambda>s. if_live_then_nonz_cap s \<and> (live_sc sc \<longrightarrow> ex_nonz_cap_to ptr s)\<rbrace>
+     update_sched_context ptr (sc_refills_update f sc) \<lbrace>\<lambda>rv. if_live_then_nonz_cap\<rbrace>"
+  by (wpsimp simp: live_sc_def)
+
+lemma set_refills_iflive[wp]:
+  "\<lbrace>if_live_then_nonz_cap\<rbrace> set_refills ptr param_b \<lbrace>\<lambda>_. if_live_then_nonz_cap\<rbrace> "
+  apply (wpsimp simp: set_refills_def get_sched_context_def wp: hoare_vcg_all_lift get_object_wp)
+  apply (clarsimp simp: if_live_then_nonz_cap_def, drule_tac x=ptr in spec)
+  apply (simp add: obj_at_def live_sc_def live_def)
+  done
+
+lemma valid_sc_sc_consumed_update[iff]:
+  "valid_sched_context (sc_consumed_update f sc) = valid_sched_context sc"
+  by (fastforce simp: valid_sched_context_def)
+
+lemma invs_consumed_time_update[iff]:
+  "invs (consumed_time_update f s) = invs s"
+  by (clarsimp simp: invs_def valid_state_def)
+
+lemma invs_cur_time_update[iff]:
+  "invs (cur_time_update f s) = invs s"
+  by (clarsimp simp: invs_def valid_state_def)
+
+lemma invs_cur_sc_update[iff]:
+  "invs (cur_sc_update f s) = invs s"
+  by (clarsimp simp: invs_def valid_state_def)
+
+lemma invs_reprogram_timer_update[iff]:
+  "invs (reprogram_timer_update f s) = invs s"
+  by (clarsimp simp: invs_def valid_state_def)
+
+lemma set_refills_zombies_final[wp]:
+  "\<lbrace>zombies_final\<rbrace> set_refills ptr param_b \<lbrace>\<lambda>_. zombies_final\<rbrace> "
+  by (wpsimp simp: set_refills_def)
+
+(* Move *)
+lemma if_fun_simp: "(\<lambda>x. if x = y then f y else f x) = f "
+  by (rule all_ext) auto
+
+lemma set_refills_valid_sc[wp]:
+   "\<lbrace>valid_sched_context sc \<rbrace>
+        set_refills ptr refills \<lbrace>\<lambda>rv. valid_sched_context sc\<rbrace>"
+ by (wpsimp wp: valid_sc_typ update_sched_context_typ_at simp: set_refills_def)
+
+lemma set_refills_refs_of [wp]:
+ "\<lbrace>\<lambda>s. P (state_refs_of s)\<rbrace>
+    set_refills ptr refills
+  \<lbrace>\<lambda>rv s. P (state_refs_of s)\<rbrace>"
+  apply (wpsimp simp: set_refills_def get_sched_context_def
+          simp_del: refs_of_defs fun_upd_apply
+          wp: get_object_wp)
+  apply (clarsimp simp: state_refs_of_def ext obj_at_def elim!: rsubst[where P = P])
+  done
+
+lemma set_refills_hyp_refs_of[wp]:
+  "\<lbrace>\<lambda>s. P (state_hyp_refs_of s)\<rbrace> set_refills ptr refills  \<lbrace>\<lambda>rv s. P (state_hyp_refs_of s)\<rbrace>"
+  by (wpsimp simp: set_refills_def)
+
+lemma set_refills_invs[wp]:
+  "\<lbrace>invs and K (length refills \<ge> 1)\<rbrace> set_refills ptr refills \<lbrace>\<lambda>_. invs\<rbrace> "
+  apply (wpsimp simp: set_refills_def invs_def valid_state_def valid_pspace_def
+                wp: valid_irq_node_typ get_sched_context_wp)
+  apply (rule conjI)
+   apply (simp add: valid_objs_def valid_obj_def obj_at_def)
+   apply (drule_tac x=ptr in bspec, fastforce)
+    apply (clarsimp simp: valid_sched_context_def)
+  apply (rule conjI)
+   apply (simp add: if_live_then_nonz_cap_def)
+   apply (drule_tac x=ptr in spec)
+   apply (simp add: obj_at_def live_def live_sc_def)
+  apply (frule (1) sym_refs_obj_atD[rotated])
+  apply clarsimp
+  apply (drule sym)
+  apply (simp only: if_fun_simp)
+  done
+
+crunches refill_split_check
+ for aligned[wp]: pspace_aligned
+ and distinct[wp]: pspace_distinct
+ and iflive[wp]: if_live_then_nonz_cap
+ and sc_at[wp]: "sc_at sc_ptr"
+ and cte_wp_at[wp]: "cte_wp_at P c"
+ and interrupt_irq_node[wp]: "\<lambda>s. P (interrupt_irq_node s)"
+ and caps_of_state[wp]: "\<lambda>s. P (caps_of_state s)"
+ and no_cdt[wp]: "\<lambda>s. P (cdt s)"
+ and no_revokable[wp]: "\<lambda>s. P (is_original_cap s)"
+ and valid_idle[wp]: valid_idle
+ and valid_irq_handlers[wp]: valid_irq_handlers
+ and valid_global_objs[wp]: "valid_global_objs"
+ and valid_global_vspace_mappings[wp]: "valid_global_vspace_mappings"
+ and valid_arch_caps[wp]: "valid_arch_caps"
+ and only_idle[wp]: "only_idle"
+ and ifunsafe[wp]: "if_unsafe_then_cap"
+ and valid_arch[wp]: "valid_arch_state"
+ and valid_irq_states[wp]: "valid_irq_states"
+ and vms[wp]: "valid_machine_state"
+ and valid_vspace_objs[wp]: "valid_vspace_objs"
+ and valid_global_refs[wp]: "valid_global_refs"
+ and v_ker_map[wp]: "valid_kernel_mappings"
+ and equal_mappings[wp]: "equal_kernel_mappings"
+ and valid_asid_map[wp]: "valid_asid_map"
+ and pspace_in_kernel_window[wp]: "pspace_in_kernel_window"
+ and cap_refs_in_kernel_window[wp]: "cap_refs_in_kernel_window"
+ and cap_refs_respects_device_region[wp]: "cap_refs_respects_device_region"
+ and pspace_respects_device_region[wp]: "pspace_respects_device_region"
+ and cur_tcb[wp]: "cur_tcb"
+ and valid_ioc[wp]: "valid_ioc"
+ and typ_at[wp]: "\<lambda>s. P (typ_at T p s)"
+  (simp: Let_def wp: hoare_drop_imps)
+
+lemma refill_split_check_zombies[wp]:
+  "\<lbrace>zombies_final\<rbrace> refill_split_check p u \<lbrace>\<lambda>rv. zombies_final\<rbrace>"
+  by (wpsimp simp: refill_split_check_def Let_def split_del: if_splits wp: hoare_drop_imp)
+
+lemma refill_split_check_ex_cap[wp]:
+  "\<lbrace>ex_nonz_cap_to p\<rbrace> refill_split_check p u \<lbrace>\<lambda>rv. ex_nonz_cap_to p\<rbrace>"
+  by (wp ex_nonz_cap_to_pres)
+
+lemma refill_split_check_mdb [wp]:
+  "\<lbrace>valid_mdb\<rbrace> refill_split_check p u  \<lbrace>\<lambda>r. valid_mdb\<rbrace>"
+  by (wpsimp wp: valid_mdb_lift)
+
+lemma refill_split_check_hyp_refs_of[wp]:
+  "\<lbrace>\<lambda>s. P (state_hyp_refs_of s)\<rbrace> refill_split_check p u \<lbrace>\<lambda>rv s. P (state_hyp_refs_of s)\<rbrace>"
+  by (wpsimp simp: refill_split_check_def Let_def split_del: if_splits wp: hoare_drop_imp)
+
+lemma refill_split_check_refs_of[wp]:
+  "\<lbrace>\<lambda>s. P (state_refs_of s)\<rbrace> refill_split_check p u \<lbrace>\<lambda>rv s. P (state_refs_of s)\<rbrace>"
+  by (wpsimp simp: refill_split_check_def Let_def split_del: if_splits wp: hoare_drop_imp)
+
+lemma refill_split_check_invs[wp]: "\<lbrace>invs\<rbrace> refill_split_check p u \<lbrace>\<lambda>rv. invs\<rbrace>"
+  apply (wpsimp simp: refill_split_check_def Let_def split_del: if_splits
+             wp: hoare_drop_imp get_sched_context_wp)
+  apply simp
+  done
+
+declare refs_of_defs[simp del]
+lemma refill_split_check_valid_sc[wp]:
+   "\<lbrace>valid_sched_context sc\<rbrace> refill_split_check p u \<lbrace>\<lambda>rv. valid_sched_context sc\<rbrace>"
+ by (wpsimp simp: refill_split_check_def Let_def split_del: if_splits
+            wp: hoare_drop_imp)
+
+lemma update_sched_context_valid_irq_node [wp]:
+  "\<lbrace>valid_irq_node\<rbrace> update_sched_context p sc  \<lbrace>\<lambda>r. valid_irq_node\<rbrace>"
+  by (wpsimp wp: valid_irq_node_typ)
+
+lemma update_sched_context_invs:
+  "\<lbrace>invs and valid_sched_context sc and (\<lambda>s. live_sc sc \<longrightarrow> ex_nonz_cap_to p s)
+     and (\<lambda>s. sym_refs ((state_refs_of s)(p := refs_of_sc sc)))\<rbrace>
+      update_sched_context p sc \<lbrace>\<lambda>rv. invs\<rbrace>"
+  by (wpsimp simp: invs_def valid_state_def valid_pspace_def simp_del: fun_upd_apply)
+
+lemma commit_time_invs: "\<lbrace>invs\<rbrace> commit_time \<lbrace>\<lambda>rv. invs\<rbrace>"
+  apply (wpsimp simp: commit_time_def simp_del: fun_upd_apply
+                wp: update_sched_context_invs)
+          apply (rule hoare_vcg_conj_lift)
+           apply (wpsimp wp: static_imp_wp simp: set_refills_def)
+          apply wpsimp
+         apply (wpsimp simp_del: fun_upd_apply)
+         apply (rule hoare_vcg_conj_lift)
+          apply (wpsimp wp: static_imp_wp)
+         apply wpsimp
+        apply (wpsimp simp: is_round_robin_def simp_del: fun_upd_apply)
+       apply (wpsimp wp: get_sched_context_wp)
+      apply (wpsimp wp: hoare_vcg_all_lift simp_del: fun_upd_apply)+
+  by (fastforce dest: invs_valid_objs invs_iflive invs_sym_refs
+       simp: valid_objs_def obj_at_def valid_obj_def if_live_then_nonz_cap_def
+             live_def live_sc_def fun_upd_idem refs_of_def state_refs_of_def)
+
+lemma refill_unblock_check_invs: "\<lbrace>invs\<rbrace> refill_unblock_check r \<lbrace>\<lambda>rv. invs\<rbrace>"
+  by (wpsimp simp: refill_unblock_check_def refills_merge_valid[simplified]
+                      is_round_robin_def
+          wp: get_refills_inv hoare_drop_imp get_sched_context_wp)
+
+crunches switch_sched_context
+  for consumed_time[wp]: "\<lambda>s. P (consumed_time s)"
+  and reprogram_timer[wp]: "\<lambda>s. P (reprogram_timer s)"
+  and cur_time[wp]: "\<lambda>s. P (cur_time s)"
+  and cur_thread[wp]: "\<lambda>s. P (cur_thread s)"
+  (wp: crunch_wps hoare_vcg_if_lift2 simp: Let_def ignore: commit_domain_time)
+
+lemma switch_sched_context_invs[wp]:
+  "\<lbrace>invs\<rbrace> switch_sched_context \<lbrace>\<lambda>_. invs \<rbrace>"
+  by (wpsimp simp: switch_sched_context_def rollback_time_def
+         wp: hoare_if gbn_inv commit_time_invs refill_unblock_check_invs
+             hoare_drop_imp hoare_vcg_if_lift2)
+
+lemma sc_and_timer_invs: "\<lbrace>invs\<rbrace> sc_and_timer \<lbrace>\<lambda>rv. invs\<rbrace>"
+  by (wpsimp simp: sc_and_timer_def)
+
 (* FIXME move *)
 lemma pred_tcb_weaken_strongerE:
   "\<lbrakk> pred_tcb_at proj P t s; \<And>tcb . P (proj tcb) \<Longrightarrow> P' (proj' tcb) \<rbrakk> \<Longrightarrow> pred_tcb_at proj' P' t s"
@@ -181,10 +576,10 @@ locale Schedule_AI_U = Schedule_AI "TYPE(unit)"
 lemma (in Schedule_AI_U) schedule_invs[wp]:
   "\<lbrace>invs\<rbrace> (Schedule_A.schedule :: (unit,unit) s_monad) \<lbrace>\<lambda>rv. invs\<rbrace>"
   apply (simp add: Schedule_A.schedule_def allActiveTCBs_def)
-  apply (wp OR_choice_weak_wp alternative_wp dmo_invs thread_get_inv
+  apply (wp OR_choice_weak_wp alternative_wp dmo_invs thread_get_inv sc_and_timer_invs
             do_machine_op_tcb select_ext_weak_wp select_wp when_def
           | clarsimp simp: getActiveTCB_def get_tcb_def)+
-  sorry
+  done
 
 (* FIXME - move *)
 lemma get_tcb_exst_update:
@@ -193,6 +588,67 @@ lemma get_tcb_exst_update:
 
 lemma ct_in_state_trans_update[simp]: "ct_in_state st (trans_state f s) = ct_in_state st s"
   apply (simp add: ct_in_state_def)
+  done
+
+(* move to Invariants_AI *)
+lemma ct_in_state_reprogram_timer_update[iff]:
+  "ct_in_state st (reprogram_timer_update f s) = ct_in_state st s"
+  by (simp add: ct_in_state_def)
+lemma ct_in_state_consumed_time_update[iff]:
+  "ct_in_state st (consumed_time_update f s) = ct_in_state st s"
+  by (simp add: ct_in_state_def)
+lemma ct_in_state_cur_time_update[iff]:
+  "ct_in_state st (cur_time_update f s) = ct_in_state st s"
+  by (simp add: ct_in_state_def)
+lemma ct_in_state_cur_sc_update[iff]:
+  "ct_in_state st (cur_sc_update f s) = ct_in_state st s"
+  by (simp add: ct_in_state_def)
+
+lemma set_refills_pred_tcb_at[wp]:
+  "\<lbrace> pred_tcb_at proj f t \<rbrace> set_refills p r \<lbrace> \<lambda>rv. pred_tcb_at proj f t \<rbrace>"
+  by (wpsimp simp: set_refills_def)
+
+lemma refill_split_check_pred_tcb_at[wp]:
+  "\<lbrace> pred_tcb_at proj f t \<rbrace> refill_split_check p u \<lbrace> \<lambda>rv. pred_tcb_at proj f t \<rbrace>"
+  by (wpsimp wp: get_sched_context_wp simp: refill_split_check_def Let_def split_del: if_splits)
+
+lemma commit_time_pred_tcb_at[wp]:
+  "\<lbrace> pred_tcb_at proj f t \<rbrace> commit_time \<lbrace> \<lambda>rv. pred_tcb_at proj f t \<rbrace>"
+  by (wpsimp simp: commit_time_def)
+
+lemma update_sched_context_ct_in_state[wp]:
+  "\<lbrace> ct_in_state t \<rbrace> update_sched_context p sc \<lbrace> \<lambda>rv. ct_in_state t \<rbrace>"
+  by (wpsimp simp: update_sched_context_def set_object_def get_object_def obj_at_def
+                      pred_tcb_at_def ct_in_state_def simp_del: fun_upd_apply) fastforce
+
+lemma set_refills_ct_in_state[wp]:
+  "\<lbrace> ct_in_state t \<rbrace> set_refills p r \<lbrace> \<lambda>rv. ct_in_state t \<rbrace>"
+  by (wpsimp simp: set_refills_def)
+
+lemma refill_split_check_ct_in_state[wp]:
+  "\<lbrace> ct_in_state t \<rbrace> refill_split_check csc consumed \<lbrace> \<lambda>rv. ct_in_state t \<rbrace>"
+  by (wpsimp simp: refill_split_check_def Let_def split_del: if_splits wp: get_sched_context_wp)
+
+lemma commit_time_ct_in_state[wp]:
+  "\<lbrace> ct_in_state t \<rbrace> commit_time \<lbrace> \<lambda>rv. ct_in_state t \<rbrace>"
+  by (wpsimp simp: commit_time_def)
+
+lemma rollback_time_ct_in_state[wp]:
+  "\<lbrace> ct_in_state t \<rbrace> rollback_time \<lbrace> \<lambda>rv. ct_in_state t \<rbrace>"
+  by (wpsimp simp: rollback_time_def)
+
+lemma refill_unblock_check_ct_in_state[wp]:
+  "\<lbrace> ct_in_state t \<rbrace> refill_unblock_check csc \<lbrace> \<lambda>rv. ct_in_state t \<rbrace>"
+  by (wpsimp wp: get_refills_wp get_sched_context_wp
+       simp: refill_unblock_check_def is_round_robin_def refills_merge_valid[simplified])
+
+lemma switch_sched_context_ct_in_state[wp]:
+  "\<lbrace> ct_in_state t \<rbrace> switch_sched_context \<lbrace> \<lambda>rv. ct_in_state t \<rbrace>"
+  by (wpsimp simp: switch_sched_context_def wp: hoare_drop_imp hoare_vcg_if_lift2)
+
+lemma sc_and_timer_activatable: "\<lbrace>ct_in_state activatable\<rbrace> sc_and_timer \<lbrace>\<lambda>rv. ct_in_state activatable\<rbrace>"
+  apply (wpsimp simp: sc_and_timer_def switch_sched_context_def
+           wp: hoare_drop_imp modify_wp hoare_vcg_if_lift2)
   done
 
 lemma (in Schedule_AI_U) schedule_ct_activateable[wp]:
@@ -206,19 +662,19 @@ lemma (in Schedule_AI_U) schedule_ct_activateable[wp]:
     done
   show ?thesis
     apply (simp add: Schedule_A.schedule_def allActiveTCBs_def)
-    apply (wp alternative_wp
+    apply (wp alternative_wp sc_and_timer_activatable
               select_ext_weak_wp select_wp stt_activatable stit_activatable
                | simp add: P Q)+
     apply (clarsimp simp: getActiveTCB_def ct_in_state_def)
-(*    apply (rule conjI)
+    apply (rule conjI)
      apply clarsimp
-     apply (case_tac "get_tcb (cur_thread s) s", simp_all add: ct_in_state_def)
+     apply (case_tac "get_tcb (cur_thread s) s", simp_all add: ct_in_state_def is_schedulable_opt_def)
      apply (drule get_tcb_SomeD)
-     apply (clarsimp simp: pred_tcb_at_def obj_at_def split: if_split_asm)
-    apply (case_tac "get_tcb x s", simp_all)
+     apply (clarsimp simp: pred_tcb_at_def obj_at_def split: if_split_asm option.split_asm)
+    apply (case_tac "get_tcb x s", simp_all add: is_schedulable_opt_def)
     apply (drule get_tcb_SomeD)
-    apply (clarsimp simp: pred_tcb_at_def obj_at_def split: if_split_asm)
-    done*) sorry
+    apply (clarsimp simp: pred_tcb_at_def obj_at_def split: if_split_asm option.split_asm)
+  done
 qed
 
 text {* invocation related lemmas *}
@@ -249,21 +705,49 @@ where
      = (\<lambda>s. sc_at scptr s
         (* probably also need something like \<and> mrefills \<le> max_extra_refills *))"
 
-
 lemma invoke_sched_context_typ_at[wp]:
   "\<lbrace>\<lambda>s. P (typ_at T p s)\<rbrace>
      invoke_sched_context i
    \<lbrace>\<lambda>rv s. P (typ_at T p s)\<rbrace>"
-(*  by (wpsimp simp: invoke_sched_context_def split: sched_context_invocation.splits)*)
-  sorry
+  by (cases i;
+      wpsimp wp: dxo_wp_weak simp: invoke_sched_context_def sched_context_bind_ntfn_def)
 
+crunch inv[wp]: refill_capacity,refill_sufficient,refill_ready "\<lambda>s. P s"
+
+lemma refill_add_tail_typ_at[wp]:
+  "\<lbrace>\<lambda>s. P (typ_at T p s)\<rbrace> refill_add_tail sc_ptr rfl \<lbrace>\<lambda>rv s. P (typ_at T p s)\<rbrace>"
+  by (wpsimp simp: refill_add_tail_def wp: get_sched_context_wp)
+
+lemma maybe_add_empty_tail_typ_at[wp]:
+  "\<lbrace>\<lambda>s. P (typ_at T p s)\<rbrace> maybe_add_empty_tail sc_ptr \<lbrace>\<lambda>rv s. P (typ_at T p s)\<rbrace>"
+  by (wpsimp simp: maybe_add_empty_tail_def wp: get_sched_context_wp)
+
+lemma refill_new_typ_at[wp]:
+  "\<lbrace>\<lambda>s. P (typ_at T p s)\<rbrace> refill_new sc_ptr new_period new_budget new_max_refills
+      \<lbrace>\<lambda>rv s. P (typ_at T p s)\<rbrace>"
+  by (wpsimp simp: refill_new_def wp: get_sched_context_wp)
+
+lemma refill_update_typ_at[wp]: (* check the definition *)
+  "\<lbrace>\<lambda>s. P (typ_at T p s)\<rbrace> refill_update sc_ptr new_period new_budget new_max_refills
+      \<lbrace>\<lambda>rv s. P (typ_at T p s)\<rbrace>"
+  by (wpsimp simp: refill_update_def wp: get_sched_context_wp)
+
+crunch typ_at[wp]: is_schedulable "P (typ_at T p s)"
+  (wp: crunch_wps select_ext_wp ignore: set_refills)
+
+lemma sched_context_resume_typ_at[wp]:
+  "\<lbrace>\<lambda>s. P (typ_at T p s)\<rbrace> sched_context_resume sc_ptr
+      \<lbrace>\<lambda>rv s. P (typ_at T p s)\<rbrace>"
+  by (wpsimp simp: sched_context_resume_def
+      wp: get_sched_context_wp hoare_vcg_if_lift2 hoare_drop_imp)
 
 lemma invoke_sched_control_typ_at[wp]:
   "\<lbrace>\<lambda>s. P (typ_at T p s)\<rbrace>
      invoke_sched_control_configure i
    \<lbrace>\<lambda>rv s. P (typ_at T p s)\<rbrace>"
-(*  by (wpsimp simp: invoke_sched_control_configure_def split: sched_control_invocation.splits)*)
-  sorry
+  by (cases i; wpsimp simp: invoke_sched_control_configure_def split_del: if_splits
+                  wp: hoare_vcg_if_lift2 hoare_drop_imp)
+
 
 lemma invoke_sched_context_tcb[wp]:
   "\<lbrace>tcb_at tptr\<rbrace> invoke_sched_context i \<lbrace>\<lambda>rv. tcb_at tptr\<rbrace>"
@@ -273,14 +757,75 @@ lemma invoke_sched_control_tcb[wp]:
   "\<lbrace>tcb_at tptr\<rbrace> invoke_sched_control_configure i \<lbrace>\<lambda>rv. tcb_at tptr\<rbrace>"
   by (simp add: tcb_at_typ invoke_sched_control_typ_at [where P=id, simplified])
 
+crunch invs[wp]: set_message_info invs
+crunches set_message_info,sched_context_update_consumed
+ for tcb_at[wp]: "tcb_at t"
+ and cur_thread[wp]: "\<lambda>s. P (cur_thread s)"
+  (wp: get_object_wp)
+
+lemma update_sched_context_tcb_at_ct[wp]:
+  "\<lbrace>\<lambda>s. tcb_at (cur_thread s) s\<rbrace> update_sched_context p sc \<lbrace>\<lambda>rv s. tcb_at (cur_thread s) s\<rbrace>"
+  by (wpsimp simp: update_sched_context_def set_object_def obj_at_def is_tcb_def wp: get_object_wp)
+
+lemma sched_context_update_consumed_tcb_at_ct[wp]:
+  "\<lbrace>\<lambda>s. tcb_at (cur_thread s) s\<rbrace> sched_context_update_consumed scp \<lbrace>\<lambda>rv s. tcb_at (cur_thread s) s\<rbrace>"
+  by (wpsimp simp: sched_context_update_consumed_def)
+
+(* RT FIXME Move *)
+lemma [simp]:
+ "live_sc (sc_consumed_update f sc) = live_sc sc"
+ "live_sc (sc_period_update f sc) = live_sc sc"
+ "live_sc (sc_refills_update g sc) = live_sc sc"
+ "live_sc (sc_badge_update h sc) = live_sc sc"
+  by (simp add: live_sc_def)+
+
+
+lemma sched_context_update_consumed_invs[wp]:
+  "\<lbrace>invs\<rbrace> sched_context_update_consumed scp \<lbrace>\<lambda>rv. invs\<rbrace>"
+  apply (wpsimp simp: sched_context_update_consumed_def wp: update_sched_context_invs get_sched_context_wp)
+  by (fastforce dest: invs_valid_objs invs_iflive invs_sym_refs
+       simp: valid_objs_def obj_at_def valid_obj_def if_live_then_nonz_cap_def
+             live_def live_sc_def fun_upd_idem refs_of_def state_refs_of_def)
+
+lemma sched_context_bind_ntfn_invs[wp]:
+  "\<lbrace>invs and sc_at sc\<rbrace> sched_context_bind_ntfn sc ntfn \<lbrace>\<lambda>rv. invs\<rbrace>"
+  apply (wpsimp simp: sched_context_bind_ntfn_def update_sk_obj_ref_def
+              wp: update_sched_context_invs get_sched_context_wp hoare_vcg_all_lift hoare_drop_imp
+             set_ntfn_minor_invs valid_sc_typ get_simple_ko_wp)
+  by (clarsimp dest: invs_valid_objs invs_iflive invs_sym_refs
+       simp: valid_objs_def obj_at_def valid_obj_def if_live_then_nonz_cap_def
+             live_def live_sc_def fun_upd_idem refs_of_def state_refs_of_def
+is_sc_obj_def split: kernel_object.splits)
+
+  sorry
+
+lemma sched_context_unbind_ntfn_invs[wp]:
+  "\<lbrace>invs\<rbrace> sched_context_unbind_ntfn sc \<lbrace>\<lambda>rv. invs\<rbrace>"
+  sorry
+
+lemma sched_context_bind_tcb_invs[wp]:
+  "\<lbrace>invs\<rbrace> sched_context_bind_tcb sc tcb \<lbrace>\<lambda>rv. invs\<rbrace>"
+   sorry
+
+lemma sched_context_unbind_tcb_invs[wp]:
+  "\<lbrace>invs\<rbrace> sched_context_unbind_tcb sc \<lbrace>\<lambda>rv. invs\<rbrace>"
+   sorry
+
+lemma sched_context_unbind_all_tcbs_invs[wp]:
+  "\<lbrace>invs\<rbrace> sched_context_unbind_all_tcbs sc \<lbrace>\<lambda>rv. invs\<rbrace>"
+   sorry
 
 lemma invoke_sched_context_invs[wp]:
   "\<lbrace>invs and valid_sched_context_inv i\<rbrace> invoke_sched_context i \<lbrace>\<lambda>rv. invs\<rbrace>"
-  sorry
+  by (cases i; wpsimp wp: dxo_wp_weak hoare_vcg_conj_lift
+          simp: invoke_sched_context_def set_consumed_def)
 
 
 lemma invoke_sched_control_configure_invs[wp]:
   "\<lbrace>invs and valid_sched_control_inv i\<rbrace> invoke_sched_control_configure i \<lbrace>\<lambda>rv. invs\<rbrace>"
+  by (cases i; wpsimp simp: invoke_sched_control_configure_def split_del: if_splits
+                  wp: hoare_vcg_if_lift2 hoare_drop_imp)
+
   sorry
 
 
@@ -305,6 +850,10 @@ lemma decode_sched_control_inv_inv:
   "\<lbrace>P\<rbrace>
      decode_sched_control_invocation label args excaps
    \<lbrace>\<lambda>rv. P\<rbrace>"
+  by (wpsimp simp: decode_sched_control_invocation_def split_del: if_splits
+             wp: hoare_vcg_if_lift2 hoare_drop_imp)
+
+
   sorry
 
 
